coq/theories/imperative/Printing.v
@@ -21,9 +21,7 @@ Definition ascii_name (n: N): option string :=
     | EmptyString => None
     | String hd _ =>
       let k := N_of_ascii hd in
-      if (N_of_ascii "0"%char <=? k)%N then
-      if (k <=? N_of_ascii "9"%char)%N then None
-      else Some s else Some s
+      if (N_of_ascii "0"%char <=? k)%N && (k <=? N_of_ascii "9"%char)%N then None else Some s
     end
   end.
 
@@ -45,250 +43,214 @@ Inductive sexpr :=
 (* Helper constructors for common s-expression patterns *)
 
 Definition unary_sexpr (op: string) (v: sexpr): sexpr :=
-  let/d op_s := SStr op in
-  let/d res := SPair op_s v in
-  let/d resb := SBlock res in
-  resb.
+  let op_s := SStr op in
+  let res := SPair op_s v in
+  SBlock res.
 
 Definition binary_sexpr (op: string) (v1 v2: sexpr): sexpr :=
-  let/d op_s := SStr op in
-  let/d args := SPair v1 v2 in
-  let/d res := SPair op_s args in
-  let/d resb := SBlock res in
-  resb.
+  let op_s := SStr op in
+  let args := SPair v1 v2 in
+  let res := SPair op_s args in
+  SBlock res.
 
 Definition ternary_sexpr (op: string) (v1 v2 v3: sexpr): sexpr :=
-  let/d op_s := SStr op in
-  let/d args1 := SPair v1 v2 in
-  let/d args := SPair args1 v3 in
-  let/d res := SPair op_s args in
-  let/d resb := SBlock res in
-  resb.
+  let op_s := SStr op in
+  let args1 := SPair v1 v2 in
+  let args := SPair args1 v3 in
+  let res := SPair op_s args in
+  SBlock res.
 
 Definition quaternary_sexpr (op: string) (v1 v2 v3 v4: sexpr): sexpr :=
-  let/d op_s := SStr op in
-  let/d args1 := SPair v1 v2 in
-  let/d args2 := SPair args1 v3 in
-  let/d args := SPair args2 v4 in
-  let/d res := SPair op_s args in
-  let/d resb := SBlock res in
-  resb.
+  let op_s := SStr op in
+  let args1 := SPair v1 v2 in
+  let args2 := SPair args1 v3 in
+  let args := SPair args2 v4 in
+  let res := SPair op_s args in
+  SBlock res.
 
-Definition name_sexpr (n: N): sexpr :=
-  let/d nm := SStr (name2str n) in
-  nm.
+Definition name_sexpr (n: N): sexpr := SStr (name2str n).
 
 Fixpoint exp2s (e: exp): sexpr :=
   match e with
   | Var n =>
-    let/d nm := name_sexpr n in
-    let/d res := unary_sexpr "var" nm in
-    res
+    let nm := name_sexpr n in
+    unary_sexpr "var" nm
   | Const w =>
-    let/d w_N := Z.to_N (word.unsigned w) in
-    let/d res := SNum w_N in
-    res
+    let w_N := Z.to_N (word.unsigned w) in
+    SNum w_N
   | Add e1 e2 =>
-    let/d v1 := exp2s e1 in
-    let/d v2 := exp2s e2 in
-    let/d res := binary_sexpr "+" v1 v2 in
-    res
+    let v1 := exp2s e1 in
+    let v2 := exp2s e2 in
+    binary_sexpr "+" v1 v2
   | Sub e1 e2 =>
-    let/d v1 := exp2s e1 in
-    let/d v2 := exp2s e2 in
-    let/d res := binary_sexpr "-" v1 v2 in
-    res
+    let v1 := exp2s e1 in
+    let v2 := exp2s e2 in
+    binary_sexpr "-" v1 v2
   | Div e1 e2 =>
-    let/d v1 := exp2s e1 in
-    let/d v2 := exp2s e2 in
-    let/d res := binary_sexpr "div" v1 v2 in
-    res
+    let v1 := exp2s e1 in
+    let v2 := exp2s e2 in
+    binary_sexpr "div" v1 v2
   | Read e1 e2 =>
-    let/d v1 := exp2s e1 in
-    let/d v2 := exp2s e2 in
-    let/d res := binary_sexpr "read" v1 v2 in
-    res
+    let v1 := exp2s e1 in
+    let v2 := exp2s e2 in
+    binary_sexpr "read" v1 v2
   end.
 
 Fixpoint exps2s_imp (es: list exp): sexpr :=
   match es with
-  | [] =>
-    let/d res := SEmpty in
-    res
+  | [] => SEmpty
   | e :: es' =>
-    let/d v := exp2s e in
-    let/d vs := exps2s_imp es' in
-    let/d res := SPair v vs in
-    res
+    let v := exp2s e in
+    let vs := exps2s_imp es' in
+    SPair v vs
   end.
 Definition exps2s (es: list exp): sexpr :=
-  let/d v := exps2s_imp es in
-  let/d res := SBlock v in
-  res.
+  let v := exps2s_imp es in
+  SBlock v.
 
 Definition cmp2str_imp (c: cmp): string :=
   match c with
-  | Less =>
-    let/d res := "<" in
-    res
-  | Equal =>
-    let/d res := "=" in
-    res
+  | Less => "<"
+  | Equal => "="
   end.
 
 Fixpoint test2s_imp (t: test): sexpr :=
   match t with
   | Test c e1 e2 =>
-    let/d cmp_str := cmp2str_imp c in
-    let/d v1 := exp2s e1 in
-    let/d v2 := exp2s e2 in
-    let/d res := binary_sexpr cmp_str v1 v2 in
-    res
+    let cmp_str := cmp2str_imp c in
+    let v1 := exp2s e1 in
+    let v2 := exp2s e2 in
+    binary_sexpr cmp_str v1 v2
   | And t1 t2 =>
-    let/d v1 := test2s_imp t1 in
-    let/d v2 := test2s_imp t2 in
-    let/d res := binary_sexpr "and" v1 v2 in
-    res
+    let v1 := test2s_imp t1 in
+    let v2 := test2s_imp t2 in
+    binary_sexpr "and" v1 v2
   | Or t1 t2 =>
-    let/d v1 := test2s_imp t1 in
-    let/d v2 := test2s_imp t2 in
-    let/d res := binary_sexpr "or" v1 v2 in
-    res
+    let v1 := test2s_imp t1 in
+    let v2 := test2s_imp t2 in
+    binary_sexpr "or" v1 v2
   | Not t' =>
-    let/d v := test2s_imp t' in
-    let/d res := unary_sexpr "not" v in
-    res
+    let v := test2s_imp t' in
+    unary_sexpr "not" v
   end.
 
 Fixpoint names2s_imp (ns: list name): sexpr :=
   match ns with
   | [] =>
-    let/d res := SEmpty in
+    let res := SEmpty in
     res
   | n :: ns' =>
-    let/d v := name_sexpr n in
-    let/d vs := names2s_imp ns' in
-    let/d res := SPair v vs in
-    res
+    let v := name_sexpr n in
+    let vs := names2s_imp ns' in
+    SPair v vs
   end.
 Definition names2s (ns: list name): sexpr :=
-  let/d v := names2s_imp ns in
-  let/d res := SBlock v in
-  res.
+  let v := names2s_imp ns in
+  SBlock v.
 
 Fixpoint cmd2s_imp (c: cmd): sexpr :=
   match c with
   | Skip =>
-    let/d res := SEmpty in
-    res
+    SEmpty
   | Seq c1 c2 =>
-    let/d v1 := cmd2s_imp c1 in
-    let/d v2 := cmd2s_imp c2 in
-    let/d res := SPair v1 v2 in
-    res
+    let v1 := cmd2s_imp c1 in
+    let v2 := cmd2s_imp c2 in
+    SPair v1 v2
   | Assign n e =>
-    let/d name_v := name_sexpr n in
-    let/d exp_v := exp2s e in
-    let/d res := binary_sexpr "assign" name_v exp_v in
-    res
+    let name_v := name_sexpr n in
+    let exp_v := exp2s e in
+    binary_sexpr "assign" name_v exp_v
   | Update a e e' =>
-    let/d addr_v := exp2s a in
-    let/d idx_v := exp2s e in
-    let/d val_v := exp2s e' in
-    let/d res := ternary_sexpr "update" addr_v idx_v val_v in
-    res
+    let addr_v := exp2s a in
+    let idx_v := exp2s e in
+    let val_v := exp2s e' in
+    ternary_sexpr "update" addr_v idx_v val_v
   | If t c1 c2 =>
-    let/d test_v := test2s_imp t in
-    let/d cmd1_v := cmd2s_imp c1 in
-    let/d cmd2_v := cmd2s_imp c2 in
-    let/d res := ternary_sexpr "if" test_v cmd1_v cmd2_v in
-    res
+    let test_v := test2s_imp t in
+    let cmd1_v := cmd2s_imp c1 in
+    let cmd2_v := cmd2s_imp c2 in
+    ternary_sexpr "if" test_v cmd1_v cmd2_v
   | While t c' =>
-    let/d test_v := test2s_imp t in
-    let/d cmd_v := cmd2s_imp c' in
-    let/d res := binary_sexpr "while" test_v cmd_v in
-    res
+    let test_v := test2s_imp t in
+    let cmd_v := cmd2s_imp c' in
+    binary_sexpr "while" test_v cmd_v
   | Call n f es =>
-    let/d name_v := name_sexpr n in
-    let/d func_v := name_sexpr f in
-    let/d args_vs := exps2s es in
-    let/d res := ternary_sexpr "call" name_v func_v args_vs in
-    res
+    let name_v := name_sexpr n in
+    let func_v := name_sexpr f in
+    let args_vs := exps2s es in
+    ternary_sexpr "call" name_v func_v args_vs
   | Return e =>
-    let/d exp_v := exp2s e in
-    let/d res := unary_sexpr "return" exp_v in
-    res
+    let exp_v := exp2s e in
+    unary_sexpr "return" exp_v
   | Alloc n e =>
-    let/d name_v := name_sexpr n in
-    let/d size_v := exp2s e in
-    let/d res := binary_sexpr "alloc" name_v size_v in
-    res
+    let name_v := name_sexpr n in
+    let size_v := exp2s e in
+    binary_sexpr "alloc" name_v size_v
   | GetChar n =>
-    let/d name_v := name_sexpr n in
-    let/d res := unary_sexpr "getchar" name_v in
-    res
+    let name_v := name_sexpr n in
+    unary_sexpr "getchar" name_v
   | PutChar e =>
-    let/d char_v := exp2s e in
-    let/d res := unary_sexpr "putchar" char_v in
-    res
+    let char_v := exp2s e in
+    unary_sexpr "putchar" char_v
   | Abort =>
-    let/d res := SStr "abort" in
-    let/d resb := SBlock res in
-    resb
+    let res := SStr "abort" in
+    SBlock res
   end.
 
 Definition func2s (f: func): sexpr :=
   match f with
   | Func n params body =>
-    let/d name_v := name_sexpr n in
-    let/d params_vs := names2s params in
-    let/d body_v := cmd2s_imp body in
-    let/d body_vb := SBlock body_v in
-    let/d res := ternary_sexpr "defun" name_v params_vs body_vb in
-    res
+    let name_v := name_sexpr n in
+    let params_vs := names2s params in
+    let body_v := cmd2s_imp body in
+    let body_vb := SBlock body_v in
+    ternary_sexpr "defun" name_v params_vs body_vb
   end.
 
 Fixpoint funcs2s_imp (fs: list func): sexpr :=
   match fs with
-  | [] =>
-    let/d res := SEmpty in
-    res
+  | [] => SEmpty
   | f :: fs' =>
-    let/d v := func2s f in
-    let/d vs := funcs2s_imp fs' in
-    let/d res := SPair v vs in
-    res
+    let v := func2s f in
+    let vs := funcs2s_imp fs' in
+    SPair v vs
   end.
 
 Definition prog2s_imp (p: prog): sexpr :=
   match p with
   | Program funcs =>
-    let/d funcs_vs := funcs2s_imp funcs in
-    funcs_vs
+    funcs2s_imp funcs
   end.
 
-Fixpoint sexpr2str (s: sexpr): string :=
+Inductive str_app_list: Type :=
+| StrList : string -> str_app_list
+| StrAppend : str_app_list -> str_app_list -> str_app_list.
+Notation "xs +++ ys" := (StrAppend xs ys) (right associativity, at level 60).
+
+Fixpoint sexpr2str (s: sexpr): str_app_list :=
   match s with
   | SNum n =>
-    let/d res := "'" ++ N2str n "" in
-    res
-  | SStr str =>
-    str
+    StrList "'" +++ StrList (N2str n "")
+  | SStr str => StrList str
   | SPair s1 s2 =>
-    let/d str1 := sexpr2str s1 in
-    let/d str2 := sexpr2str s2 in
-    let/d res := str1 ++ " " ++ str2 in
-    res
-  | SEmpty =>
-    let/d res := "" in
-    res
+    let str1 := sexpr2str s1 in
+    let str2 := sexpr2str s2 in
+    str1 +++ StrList " " +++ str2
+  | SEmpty => StrList ""
   | SBlock s' =>
-    let/d str' := sexpr2str s' in
-    let/d res := "(" ++ str' ++ ")" in
-    res
+    let str' := sexpr2str s' in
+    StrList "(" +++ str' +++ StrList ")"
+  end.
+
+Fixpoint flatten_str_app_list (sal: str_app_list): string :=
+  match sal with
+  | StrList s => s
+  | StrAppend sal1 sal2 =>
+    let s1 := flatten_str_app_list sal1 in
+    let s2 := flatten_str_app_list sal2 in
+    s1 ++ s2
   end.
 
 Definition imp2str (p: prog): string :=
-  let/d v := prog2s_imp p in
-  let/d res := sexpr2str v in
-  res.
+  let v := prog2s_imp p in
+  flatten_str_app_list (sexpr2str v).
