coq/theories/bootstrapping/Bootstrapping.v
@@ -1,6 +1,5 @@
 From impboot Require Import
   Core
-  imperative.Printing
   derivations.AsmToStringDerivations
   derivations.ParserDerivations
   derivations.CompilerUtilsDerivations
@@ -25,64 +24,3 @@ Time Eval lazy in compiler_program_asm.
 Definition compiler_asm_str := asm2str compiler_program_asm.
 
 Time Eval lazy in compiler_asm_str.
-
-(* Definition get_fun_name (f: FunSyntax.defun): N :=
-  match f with
-  | FunSyntax.Defun n _ _ => n
-  end.
-
-Definition compiler_funs_imp :=
-  List.map (fun f => (N2ascii_default (get_fun_name f), to_funs [f])) (read_inp_prog :: print_string_prog :: compiler_funs).
-
-Eval lazy in compiler_funs_imp. *)
-
-(* 
-Definition compiler_funs_imp1 :=
-  List.map (fun f => (N2ascii (get_fun_name f), to_funs [f])) (read_inp_prog :: print_string_prog :: firstn 5 compiler_funs).
-
-(* Eval lazy in compiler_funs_imp1. *)
-
-Print v2exp_prog.
-Eval lazy in to_cmd (
-  (FunSyntax.Call
-  (FunValues.name_enc "vel0")
-  [FunSyntax.Op
-    FunSyntax.Cons
-    [FunSyntax.Const
-      (FunValues.name_enc "Pair");
-      FunSyntax.Op
-      FunSyntax.Cons
-      [FunSyntax.Var
-      (FunValues.name_enc "v1");
-      FunSyntax.Op
-      FunSyntax.Cons
-      [FunSyntax.Op
-      FunSyntax.Cons
-      [FunSyntax.Const
-      (FunValues.name_enc "Pair");
-      FunSyntax.Op
-      FunSyntax.Cons
-      [FunSyntax.Var
-      (FunValues.name_enc "v3");
-      FunSyntax.Op
-      FunSyntax.Cons
-      [FunSyntax.Op
-      FunSyntax.Cons
-      [FunSyntax.Const
-      (FunValues.name_enc "Pair");
-      FunSyntax.Op
-      FunSyntax.Cons
-      [FunSyntax.Var
-      (FunValues.name_enc "v5");
-      FunSyntax.Op
-      FunSyntax.Cons
-      [FunSyntax.Var
-      (FunValues.name_enc "v6");
-      FunSyntax.Const 0]]];
-      FunSyntax.Const 0]]];
-    FunSyntax.Const 0]]]
-  ]
-  )
-). *)
-
-(* Eval lazy in to_imp compiler_program_prog. *)
