coq/theories/derivations/CompilerUtilsDerivations.v
@@ -20,23 +20,32 @@ From Stdlib Require Import derive.Derive.
 From Stdlib Require Import Lia.
 From Ltac2 Require Import Ltac2.
 
-Derive nat_modulo_prog
-  in ltac2:(relcompile_tpe 'nat_modulo_prog 'nat_modulo ['mul_nat]) 
-  as nat_modulo_prog_proof.
+Derive nat_modulo_10_prog
+  in ltac2:(relcompile_tpe 'nat_modulo_10_prog 'nat_modulo_10 ['mul_nat_10])
+  as nat_modulo_10_prog_proof.
 Proof.
   time relcompile.
   ltac1:(lia).
 Qed.
-Time Compute to_funs [nat_modulo_prog].
+Time Compute to_funs [nat_modulo_10_prog].
 
-Derive N_modulo_prog
-  in ltac2:(relcompile_tpe 'N_modulo_prog 'N_modulo ['mul_N]) 
-  as N_modulo_prog_proof.
+Derive N_modulo_10_prog
+  in ltac2:(relcompile_tpe 'N_modulo_10_prog 'N_modulo_10 ['mul_N_10])
+  as N_modulo_10_prog_proof.
 Proof.
   time relcompile.
   ltac1:(lia).
 Qed.
-Time Compute to_funs [nat_modulo_prog].
+Time Compute to_funs [N_modulo_10_prog].
+
+Derive N_modulo_256_prog
+  in ltac2:(relcompile_tpe 'N_modulo_256_prog 'N_modulo_256 ['mul_N_256])
+  as N_modulo_256_prog_proof.
+Proof.
+  time relcompile.
+  ltac1:(lia).
+Qed.
+Time Compute to_funs [N_modulo_256_prog].
 
 Theorem string_append_equation: ltac2:(unfold_fix_type '@string_append).
 Proof. unfold_fix_proof '@string_append. Qed.
@@ -46,18 +55,18 @@ Derive string_append_prog
 Proof.
   time relcompile.
 Qed.
-Time Compute to_funs [nat_modulo_prog].
+Time Compute to_funs [string_append_prog].
 
 Theorem num2str_f_equation: ltac2:(unfold_fix_type '@num2str_f).
 Proof. unfold_fix_proof '@num2str_f. Qed.
 
 Derive num2str_f_prog
-  in ltac2:(relcompile_tpe 'num2str_f_prog 'num2str_f ['nat_modulo])
+  in ltac2:(relcompile_tpe 'num2str_f_prog 'num2str_f ['nat_modulo_10])
   as num2str_f_prog_proof.
 Proof.
   time relcompile.
   all: ltac1:(try lia).
-  all: subst; specialize nat_modulo_le with (n := n) (m := 10); ltac1:(lia).
+  all: subst; rewrite nat_modulo_10_spec in *; specialize nat_modulo_le with (n := n) (m := 10); ltac1:(lia).
 Qed.
 Time Compute to_funs [num2str_f_prog].
 
@@ -73,13 +82,13 @@ Theorem N2str_f_equation: ltac2:(unfold_fix_type '@N2str_f).
 Proof. unfold_fix_proof '@N2str_f. Qed.
 
 Derive N2str_f_prog
-  in ltac2:(relcompile_tpe 'N2str_f_prog 'N2str_f ['N_modulo])
+  in ltac2:(relcompile_tpe 'N2str_f_prog 'N2str_f ['N_modulo_10])
   as N2str_f_prog_proof.
 Proof.
   time relcompile.
   all: ltac1:(try lia).
   all: rewrite ?N.ltb_lt in *; ltac1:(try lia).
-  all: subst; specialize N_modulo_le with (n := n) (m := 10%N) as ?; ltac1:(try lia).
+  all: subst; rewrite N_modulo_10_spec in *; specialize N_modulo_le with (n := n) (m := 10%N) as ?; ltac1:(try lia).
 Qed.
 Time Compute to_funs [N2str_f_prog].
 
@@ -136,43 +145,47 @@ Proof.
 Qed.
 Time Compute to_funs [app_list_length_prog].
 
-Theorem mul_nat_equation: ltac2:(unfold_fix_type '@mul_nat).
-Proof. unfold_fix_proof '@mul_nat. Qed.
-Derive mul_nat_prog
-  in ltac2:(relcompile_tpe 'mul_nat_prog 'mul_nat [])
-  as mul_nat_prog_proof.
+Derive mul_N_10_prog
+  in ltac2:(relcompile_tpe 'mul_N_10_prog 'mul_N_10 [])
+  as mul_N_10_prog_proof.
 Proof.
   time relcompile.
 Qed.
-Time Compute to_funs [mul_nat_prog].
+Time Compute to_funs [mul_N_10_prog].
 
-Theorem mul_N_f_equation: ltac2:(unfold_fix_type '@mul_N_f).
-Proof. unfold_fix_proof '@mul_N_f. Qed.
-Derive mul_N_f_prog
-  in ltac2:(relcompile_tpe 'mul_N_f_prog 'mul_N_f [])
-  as mul_N_f_prog_proof.
+Derive mul_N_256_prog
+  in ltac2:(relcompile_tpe 'mul_N_256_prog 'mul_N_256 [])
+  as mul_N_256_prog_proof.
 Proof.
   time relcompile.
 Qed.
-Time Compute to_funs [mul_N_f_prog].
+Time Compute to_funs [mul_N_256_prog].
 
-Derive mul_N_prog
-  in ltac2:(relcompile_tpe 'mul_N_prog 'mul_N ['mul_N_f])
-  as mul_N_prog_proof.
+Derive mul_nat_8_prog
+  in ltac2:(relcompile_tpe 'mul_nat_8_prog 'mul_nat_8 [])
+  as mul_nat_8_prog_proof.
 Proof.
   time relcompile.
 Qed.
-Time Compute to_funs [mul_N_prog].
+Time Compute to_funs [mul_nat_8_prog].
+
+Derive mul_nat_10_prog
+  in ltac2:(relcompile_tpe 'mul_nat_10_prog 'mul_nat_10 [])
+  as mul_nat_10_prog_proof.
+Proof.
+  time relcompile.
+Qed.
+Time Compute to_funs [mul_nat_10_prog].
 
 Theorem N2ascii_f_equation: ltac2:(unfold_fix_type '@N2ascii_f).
 Proof. unfold_fix_proof '@N2ascii_f. Qed.
 Derive N2ascii_f_prog
-  in ltac2:(relcompile_tpe 'N2ascii_f_prog 'N2ascii_f ['N_modulo; 'string_append])
+  in ltac2:(relcompile_tpe 'N2ascii_f_prog 'N2ascii_f ['N_modulo_256; 'string_append])
   as N2ascii_f_prog_proof.
 Proof.
   time relcompile.
   all: ltac1:(try lia).
-  all: subst; specialize N_modulo_lt with (n := n) (m := 256%N) as ?; ltac1:(try lia).
+  all: subst; rewrite N_modulo_256_spec in *; specialize N_modulo_lt with (n := n) (m := 256%N) as ?; ltac1:(try lia).
 Qed.
 Time Compute to_funs [N2ascii_f_prog].
 
@@ -194,11 +207,13 @@ Qed.
 Time Compute to_funs [N2ascii_default_prog].
 
 Definition CompilerUtils_funs := [
-  mul_nat_prog;
-  mul_N_f_prog;
-  mul_N_prog;
-  nat_modulo_prog;
-  N_modulo_prog;
+  mul_nat_8_prog;
+  mul_nat_10_prog;
+  mul_N_10_prog;
+  mul_N_256_prog;
+  nat_modulo_10_prog;
+  N_modulo_10_prog;
+  N_modulo_256_prog;
   num2str_f_prog;
   num2str_prog;
   N2str_f_prog;
@@ -229,20 +244,22 @@ Ltac2 assert_eval_app_by (fname: constr) (prf: constr) (list_constr_hyp: constr)
   ).
 
 Ltac2 assert_eval_app_compiler_utils (hlookup_constr: constr) :=
-  assert_eval_app_by 'mul_nat 'mul_nat_prog_proof hlookup_constr 0;
-  assert_eval_app_by 'mul_N_f 'mul_N_f_prog_proof hlookup_constr 1;
-  assert_eval_app_by 'mul_N 'mul_N_prog_proof hlookup_constr 2;
-  assert_eval_app_by 'nat_modulo 'nat_modulo_prog_proof hlookup_constr 3;
-  assert_eval_app_by 'N_modulo 'N_modulo_prog_proof hlookup_constr 4;
-  assert_eval_app_by 'num2str_f 'num2str_f_prog_proof hlookup_constr 5;
-  assert_eval_app_by 'num2str 'num2str_prog_proof hlookup_constr 6;
-  assert_eval_app_by 'N2str_f 'N2str_f_prog_proof hlookup_constr 7;
-  assert_eval_app_by 'N2str 'N2str_prog_proof hlookup_constr 8;
-  assert_eval_app_by '@list_length 'list_length_prog_proof hlookup_constr 9;
-  assert_eval_app_by '@list_append 'list_append_prog_proof hlookup_constr 10;
-  assert_eval_app_by '@flatten 'flatten_prog_proof hlookup_constr 11;
-  assert_eval_app_by '@app_list_length 'app_list_length_prog_proof hlookup_constr 12;
-  assert_eval_app_by 'string_append 'string_append_prog_proof hlookup_constr 13;
-  assert_eval_app_by 'N2ascii_f 'N2ascii_f_prog_proof hlookup_constr 14;
-  assert_eval_app_by 'N2ascii 'N2ascii_prog_proof hlookup_constr 15;
-  assert_eval_app_by 'N2ascii_default 'N2ascii_default_prog_proof hlookup_constr 16.
+  assert_eval_app_by 'mul_nat_8 'mul_nat_8_prog_proof hlookup_constr 0;
+  assert_eval_app_by 'mul_nat_10 'mul_nat_10_prog_proof hlookup_constr 1;
+  assert_eval_app_by 'mul_N_10 'mul_N_10_prog_proof hlookup_constr 2;
+  assert_eval_app_by 'mul_N_256 'mul_N_256_prog_proof hlookup_constr 3;
+  assert_eval_app_by 'nat_modulo_10 'nat_modulo_10_prog_proof hlookup_constr 4;
+  assert_eval_app_by 'N_modulo_10 'N_modulo_10_prog_proof hlookup_constr 5;
+  assert_eval_app_by 'N_modulo_256 'N_modulo_256_prog_proof hlookup_constr 6;
+  assert_eval_app_by 'num2str_f 'num2str_f_prog_proof hlookup_constr 7;
+  assert_eval_app_by 'num2str 'num2str_prog_proof hlookup_constr 8;
+  assert_eval_app_by 'N2str_f 'N2str_f_prog_proof hlookup_constr 9;
+  assert_eval_app_by 'N2str 'N2str_prog_proof hlookup_constr 10;
+  assert_eval_app_by '@list_length 'list_length_prog_proof hlookup_constr 11;
+  assert_eval_app_by '@list_append 'list_append_prog_proof hlookup_constr 12;
+  assert_eval_app_by '@flatten 'flatten_prog_proof hlookup_constr 13;
+  assert_eval_app_by '@app_list_length 'app_list_length_prog_proof hlookup_constr 14;
+  assert_eval_app_by 'string_append 'string_append_prog_proof hlookup_constr 15;
+  assert_eval_app_by 'N2ascii_f 'N2ascii_f_prog_proof hlookup_constr 16;
+  assert_eval_app_by 'N2ascii 'N2ascii_prog_proof hlookup_constr 17;
+  assert_eval_app_by 'N2ascii_default 'N2ascii_default_prog_proof hlookup_constr 18.
