coq/theories/imp2asm/CompilerProofs.v
@@ -1,0 +1,15 @@
+From impboot.utils Require Import Core.
+From impboot.imp2asm Require Import Compiler.
+From impboot.parsing Require Import Parser.
+From impboot.imperative Require Import Printing.
+From impboot.bootstrapping Require Import Bootstrapping.
+
+Theorem print_parser_compiler_correct:
+  match compiler_program_imp with
+  | None => False
+  | Some compiler_imp =>
+    compiler_imp = str2imp (list_ascii_of_string (imp2str compiler_imp))
+  end.
+Proof.
+  lazy; reflexivity.
+Qed.
